@prefix at-voc: <http://publications.europa.eu/resource/authority/> .
@prefix cccev: <http://data.europa.eu/m8g/> .
@prefix dcterms: <http://purl.org/dc/terms/> .
@prefix esco: <http://data.europa.eu/esco/model#> .
@prefix foaf: <http://xmlns.com/foaf/0.1/> .
@prefix locn: <http://www.w3.org/ns/locn#> .
@prefix org: <http://www.w3.org/ns/org#> .
@prefix owl: <http://www.w3.org/2002/07/owl#> .
@prefix rdf: <http://www.w3.org/1999/02/22-rdf-syntax-ns#> .
@prefix rdfs: <http://www.w3.org/2000/01/rdf-schema#> .
@prefix rmo: <http://index.dev/ontology/rmo#> .
@prefix skos: <http://www.w3.org/2004/02/skos/core#> .
@prefix vann: <http://purl.org/vocab/vann/> .
@prefix xsd: <http://www.w3.org/2001/XMLSchema#> .

esco:Occupation a owl:NamedIndividual,
        skos:ConceptScheme ;
    skos:prefLabel "Occupation"@en .

esco:Qualification a owl:NamedIndividual,
        skos:ConceptScheme ;
    skos:prefLabel "Qualification"@en .

esco:Skill a owl:NamedIndividual,
        skos:ConceptScheme ;
    skos:prefLabel "Skill"@en .

rmo:BenefitName a owl:DatatypeProperty ;
    rdfs:isDefinedBy rmo:tech ;
    skos:prefLabel "Benefit name"@en .

rmo:Benefits a owl:Class ;
    rdfs:isDefinedBy rmo:tech ;
    skos:definition "Additional advantages provided to employees beyond their salary, such as health insurance or retirement plans."@en ;
    skos:prefLabel "Benefits"@en .

rmo:Candidate a owl:Class ;
    rdfs:isDefinedBy rmo:tech ;
    skos:definition "An individual who uses the system to find job opportunities."@en ;
    skos:prefLabel "Candidate"@en .

rmo:CandidateProfile a owl:Class ;
    rdfs:isDefinedBy rmo:tech ;
    skos:definition "Represents the detailed profile of a Candidate, including credentials, skills experience, and location."@en ;
    skos:prefLabel "Candidate profile"@en .

rmo:Certification a owl:Class ;
    rdfs:isDefinedBy rmo:tech ;
    rdfs:subClassOf rmo:Credential ;
    skos:definition "The official recognition of a candidate's expertise or proficiency in a specific domain, typically obtained through examination or evaluation by a professional body."@en ;
    skos:prefLabel "Certification"@en .

rmo:Company a owl:Class ;
    rdfs:isDefinedBy rmo:tech ;
    skos:definition "An organization or business entity that employs individuals."@en ;
    skos:prefLabel "Company"@en .

rmo:Education a owl:Class ;
    rdfs:isDefinedBy rmo:tech ;
    rdfs:subClassOf rmo:Credential ;
    skos:definition "The academic qualifications of a Candidate."@en ;
    skos:prefLabel "Education"@en .

rmo:Experience a owl:Class ;
    rdfs:isDefinedBy rmo:tech ;
    skos:definition "Represents the practical knowledge and proficiency gained by a candidate through previous work engagements, projects, or hands-on activities."@en ;
    skos:prefLabel "Experience"@en .

rmo:JobDescription a owl:Class ;
    rdfs:isDefinedBy rmo:tech ;
    skos:definition "A job opening posted by a company, including job details and requirements."@en ;
    skos:prefLabel "Job description"@en .

rmo:Qualification a owl:Class ;
    rdfs:isDefinedBy rmo:tech ;
    rdfs:subClassOf skos:Concept ;
    skos:definition "Qualifications are the formal outcome of an assessment and validation process by a competent body determining that an individual has achieved learning outcomes to given standards."@en ;
    skos:prefLabel "Qualification"@en .

rmo:Role a owl:Class ;
    rdfs:isDefinedBy rmo:tech ;
    rdfs:subClassOf skos:Concept ;
    skos:definition "Represents the specific job occupations, positions, or professions for which candidates may be qualified or seeking employment opportunities."@en ;
    skos:prefLabel "Role"@en .

rmo:Skill a owl:Class ;
    rdfs:isDefinedBy rmo:tech ;
    rdfs:subClassOf skos:Concept ;
    skos:definition "A specific capability or proficiency possessed by a candidate, often acquired through training, practice, or experience."@en ;
    skos:prefLabel "Skill"@en .

rmo:TypeOfEngagement a owl:Class ;
    rdfs:isDefinedBy rmo:tech ;
    skos:definition "Represents various arrangements under which individuals are employed, such as part-time, full-time, or contractual roles."@en ;
    skos:prefLabel "Type of engagement"@en .

rmo:availability a owl:DatatypeProperty ;
    rdfs:isDefinedBy rmo:tech ;
    skos:definition "Indicates when the job position is open for applications, including specific dates or time frames such as \"immediate\" or \"within three months.\" (rmo:JobDescription)"@en ;
    skos:prefLabel "Availability"@en .

rmo:companyName a owl:DatatypeProperty ;
    rdfs:isDefinedBy rmo:tech ;
    skos:definition "The name of the organization or business entity that has posted a job description. (rmo:Company)"@en ;
    skos:prefLabel "Company name"@en .

rmo:dateAwarded a owl:DatatypeProperty ;
    rdfs:isDefinedBy rmo:tech ;
    skos:definition "The date when a candidate was granted a particular credential, such as a degree or certification. (rmo:Credential)"@en ;
    skos:prefLabel "Date awarded"@en .

rmo:educationDegree a owl:DatatypeProperty ;
    rdfs:isDefinedBy rmo:tech ;
    skos:prefLabel "Education degree"@en .

rmo:engagementType a owl:DatatypeProperty ;
    rdfs:isDefinedBy rmo:tech ;
    skos:definition "It includes part-time, full-time, or contractual roles. (rmo:TypeOfEngagement)"@en ;
    skos:prefLabel "Engagement type"@en .

rmo:essentialFor a owl:ObjectProperty ;
    rdfs:isDefinedBy rmo:tech ;
    skos:definition "Indicates that a particular resource or characteristic is necessary or crucial for a specific entity or concept within the ontology in order to fulfill its intended purpose. (rmo:Skill -> rmo:Role (+rmo:essentialFor))"@en ;
    skos:prefLabel "Essential for"@en .

rmo:hasBenefits a owl:ObjectProperty ;
    rdfs:isDefinedBy rmo:tech ;
    skos:definition "Indicates the benefits associated with a specific type of job engagement. (rmo:TypeOfEngagement -> rmo:Benefits (+rmo:hasBenefits))"@en ;
    skos:prefLabel "Has benefits"@en .

rmo:hasCredential a owl:ObjectProperty ;
    rdfs:isDefinedBy rmo:tech ;
    skos:definition "Academic qualifications and professional certifications obtained by a candidate. (rmo:CandidateProfile -> rmo:Credential (+rmo:hasCredential))"@en ;
    skos:prefLabel "Has credential"@en .

rmo:hasEngagement a owl:ObjectProperty ;
    rdfs:isDefinedBy rmo:tech ;
    skos:definition "Indicates what type of engagement a specific job description entails. (rmo:JobDescription -> rmo:TypeOfEngagement (+rmo:hasEngagement))"@en ;
    skos:prefLabel "Has engagement"@en .

rmo:hasExperience a owl:ObjectProperty ;
    rdfs:isDefinedBy rmo:tech ;
    skos:definition "Represents the work experience details of a candidate profile. (rmo:CandidateProfile -> rmo:Experience (+rmo:hasExperience))"@en ;
    skos:prefLabel "Has experience"@en .

rmo:hasLocation a owl:ObjectProperty ;
    rdfs:isDefinedBy rmo:tech ;
    skos:definition "Specifies the geographical location and time zone relevant to candidate profile. (rmo:Company -> dct:Location (+rmo:hasLocation)) Specifies the geographical location and timezone relevant to CandidateProfile. (rmo:CandidateProfile -> dct:Location (+rmo:hasLocation))"@en ;
    skos:prefLabel "Has location"@en .

rmo:hasProfile a owl:ObjectProperty ;
    rdfs:isDefinedBy rmo:tech ;
    skos:definition "Indicates the candidate profile of a specific Candidate. (rmo:Candidate -> rmo:CandidateProfile (+rmo:hasProfile))"@en ;
    skos:prefLabel "Has profile"@en .

rmo:hasQualification a owl:ObjectProperty ;
    rdfs:isDefinedBy rmo:tech ;
    skos:prefLabel "Has qualification"@en .

rmo:hasSkillUsed a owl:ObjectProperty ;
    rdfs:isDefinedBy rmo:tech ;
    skos:definition "Indicates that a specific skill was utilized in a particular experience. (rmo:Experience -> rmo:Skill (+rmo:hasSkillUsed))"@en ;
    skos:prefLabel "Has skill used"@en .

rmo:hasSkills a owl:ObjectProperty ;
    rdfs:isDefinedBy rmo:tech ;
    skos:definition "Indicates that a candidate profile possesses a specific skill. (rmo:CandidateProfile -> rmo:Skill (+rmo:hasSkills))"@en ;
    skos:prefLabel "Has skills"@en .

rmo:industry a owl:DatatypeProperty ;
    rdfs:isDefinedBy rmo:tech ;
    skos:prefLabel "Industry"@en .

rmo:isRelatedTo a owl:ObjectProperty ;
    rdfs:isDefinedBy rmo:tech ;
    skos:definition "Indicates that a specific resource is associated with a particular other resource. (rmo:Experience -> rmo:Role (+rmo:isRelatedTo)) Indicates that a specific resource is associated with a particular other resource. (rmo:Experience -> rmo:Qualification (+rmo:isRelatedTo))"@en ;
    skos:prefLabel "Is related to"@en .

rmo:jobId a owl:DatatypeProperty ;
    rdfs:isDefinedBy rmo:tech ;
    skos:definition "A unique identifier for a job description, used to distinguish it from other job description. (rmo:JobDescription)"@en ;
    skos:prefLabel "Job id"@en .

rmo:offersPosition a owl:ObjectProperty ;
    rdfs:isDefinedBy rmo:tech ;
    skos:definition "Indicates the job position offered by a job description. (rmo:JobDescription -> rmo:Role (+rmo:offersPosition))"@en ;
    skos:prefLabel "Offers position"@en .

rmo:optionalFor a owl:ObjectProperty ;
    rdfs:isDefinedBy rmo:tech ;
    skos:definition "Indicates that a particular resource or characteristic is optional or non-compulsory for a specific entity or concept within the ontology. (rmo:Skill -> rmo:Role (+rmo:optionalFor))"@en ;
    skos:prefLabel "Optional for"@en .

rmo:phoneNumber a owl:DatatypeProperty ;
    rdfs:isDefinedBy rmo:tech ;
    skos:definition "A telephone number through which the Candidate can be contacted. (rmo:Candidate)"@en ;
    skos:prefLabel "Phone number"@en .

rmo:posts a owl:ObjectProperty ;
    rdfs:isDefinedBy rmo:tech ;
    skos:definition "Indicates that a Company publishes a job description. (rmo:Company -> rmo:JobDescription (+rmo:posts))"@en ;
    skos:prefLabel "Posts"@en .

rmo:profileId a owl:DatatypeProperty ;
    rdfs:isDefinedBy rmo:tech ;
    skos:definition "A unique identifier for the candidate profile. (rmo:CandidateProfile)"@en ;
    skos:prefLabel "Profile id"@en .

rmo:projectType a owl:DatatypeProperty ;
    rdfs:isDefinedBy rmo:tech ;
    skos:definition "Represents the nature or category of a project, such as software development, research, or marketing. (rmo:JobDescription)"@en ;
    skos:prefLabel "Project type"@en .

rmo:rate a owl:DatatypeProperty ;
    rdfs:isDefinedBy rmo:tech ;
    skos:definition "Specifies the compensation for the job, typically expressed as an hourly rate, salary, or contract amount. (rmo:JobDescription)"@en ;
    skos:prefLabel "Rate"@en .

rmo:receivesJobDesciption a owl:ObjectProperty ;
    rdfs:isDefinedBy rmo:tech ;
    skos:definition "Indicates that a candidate profile receives a job description from the system. (rmo:CandidateProfile -> rmo:JobDescription (+rmo:receivesJobDesciption))"@en ;
    skos:prefLabel "Receives job desciption"@en .

rmo:requiresCredential a owl:ObjectProperty ;
    rdfs:isDefinedBy rmo:tech ;
    skos:definition "Indicates that a job description may require one or more Academic qualifications and/or professional certifications. (rmo:JobDescription -> rmo:Credential (+rmo:requiresCredential))"@en ;
    skos:prefLabel "Requires credential"@en .

rmo:requiresExperience a owl:ObjectProperty ;
    rdfs:isDefinedBy rmo:tech ;
    skos:definition "Specifies the type and level of experience required for a job description. (rmo:JobDescription -> rmo:Experience (+rmo:requiresExperience))"@en ;
    skos:prefLabel "Requires experience"@en .

rmo:requiresQualification a owl:ObjectProperty ;
    rdfs:isDefinedBy rmo:tech ;
    skos:definition "Specifies the qualifications required for a job description. (rmo:JobDescription -> rmo:Qualification (+rmo:requiresQualification))"@en ;
    skos:prefLabel "Requires qualification"@en .

rmo:requiresSkill a owl:ObjectProperty ;
    rdfs:isDefinedBy rmo:tech ;
    skos:definition "Specifies the skills that are necessary for a job description. (rmo:JobDescription -> rmo:Skill (+rmo:requiresSkill))"@en ;
    skos:prefLabel "Requires skill"@en .

rmo:specifiesLocation a owl:ObjectProperty ;
    rdfs:isDefinedBy rmo:tech ;
    skos:definition "Specifies the geographical location and time zone relevant to job description. (rmo:JobDescription -> dct:Location (+rmo:specifiesLocation))"@en ;
    skos:prefLabel "Specifies location"@en .

rmo:startDate a rdf:Property ;
    rdfs:isDefinedBy rmo:tech ;
    skos:definition "Represents the date when a job description, project, or engagement is scheduled to begin. (rmo:JobDescription)"@en ;
    skos:prefLabel "Start date"@en .

rmo:targetOccupation a owl:ObjectProperty ;
    rdfs:isDefinedBy rmo:tech ;
    skos:definition "Indicates the job roles or occupations that a candidate profile is interested in or qualified for. (rmo:CandidateProfile -> rmo:Role (+rmo:targetOccupation))"@en ;
    skos:prefLabel "Target occupation"@en .

rmo:targetRate a owl:DatatypeProperty ;
    rdfs:isDefinedBy rmo:tech ;
    skos:definition "Specifies the desired hourly or annual rate of pay for the candidate, indicating their expected compensation for a job. (rmo:CandidateProfile)"@en ;
    skos:prefLabel "Target rate"@en .

rmo:timeZone a owl:DatatypeProperty ;
    rdfs:isDefinedBy rmo:tech ;
    skos:definition "An area which observes a uniform standard time for legal, commercial and social purposes. (dct:Location)"@en ;
    skos:prefLabel "Time zone"@en .

rmo:yearsOfExperience a rdf:Property ;
    rdfs:isDefinedBy rmo:tech ;
    skos:definition "Indicates the total number of years a candidate has worked in their field or occupation. (rmo:Experience)"@en ;
    skos:prefLabel "Years of experience"@en .

rmo:yearsOfSkill a owl:DatatypeProperty ;
    rdfs:isDefinedBy rmo:tech ;
    skos:definition "Indicates the number of years a candidate has utilized a specific skill. (rmo:Skill)"@en ;
    skos:prefLabel "Years of skill"@en .

dcterms:Location a owl:Class ;
    skos:definition "A geographic area or place characterized by its physical coordinates and corresponding time zone."@en ;
    skos:prefLabel "Location"@en .

dcterms:description a owl:DatatypeProperty ;
    skos:definition "An account of the resource. Additional Information: Description may include but is not limited to: an abstract, a table of contents, a graphical representation, or a free-text account of the resource. (rmo:Benefits) An account of the resource. Additional Information: Description may include but is not limited to: an abstract, a table of contents, a graphical representation, or a free-text account of the resource. (rmo:Certification) An account of the resource. Additional Information: Description may include but is not limited to: an abstract, a table of contents, a graphical representation, or a free-text account of the resource. (rmo:Company) An account of the resource. Additional Information: Description may include but is not limited to: an abstract, a table of contents, a graphical representation, or a free-text account of the resource. (rmo:Experience) An account of the resource. Additional Information: Description may include but is not limited to: an abstract, a table of contents, a graphical representation, or a free-text account of the resource. (rmo:JobDescription) An account of the resource. Additional Information: Description may include but is not limited to: an abstract, a table of contents, a graphical representation, or a free-text account of the resource. (rmo:Qualification)"@en ;
    skos:prefLabel "Description"@en .

dcterms:title a owl:DatatypeProperty ;
    skos:definition "Represents the title or the name of a resource. (rmo:Candidate) Represents the title or the name of a resource. (rmo:Credential) Represents the title or the name of a resource. (rmo:Experience) Represents the title or the name of a resource. (rmo:JobDescription) Represents the title or the name of a resource. (rmo:Qualification) Represents the title or the name of a resource. (rmo:Role) Represents the title or the name of a resource. (rmo:Skill)"@en ;
    skos:prefLabel "Title"@en .

skos:altLabel a owl:DatatypeProperty ;
    skos:definition "An alternative lexical label for a resource. Acronyms, abbreviations, spelling variants, and irregular plural/singular forms may be included among the alternative labels for a concept. (rmo:Qualification) An alternative lexical label for a resource. Acronyms, abbreviations, spelling variants, and irregular plural/singular forms may be included among the alternative labels for a concept. (rmo:Skill) An alternative lexical label for a resource. Acronyms, abbreviations, spelling variants, and irregular plural/singular forms may be included among the alternative labels for a concept. (rmo:TypeOfEngagement)"@en ;
    skos:prefLabel "Alt label"@en .

skos:inScheme a owl:ObjectProperty ;
    skos:definition "A Concept Scheme in which the Concept is included. A Concept may be a member of more than one concept scheme. (rmo:Qualification -> esco:Qualification (+skos:inScheme)) A Concept Scheme in which the Concept is included. A Concept may be a member of more than one concept scheme. (rmo:Role -> esco:Occupation (+skos:inScheme)) A Concept Scheme in which the Concept is included. A Concept may be a member of more than one concept scheme. (rmo:Skill -> esco:Skill (+skos:inScheme))"@en ;
    skos:prefLabel "In scheme"@en .

skos:prefLabel a rdf:Property ;
    skos:definition "The preferred lexical label for a resource, in a given language. (rmo:Qualification) The preferred lexical label for a resource, in a given language. (rmo:Skill)"@en ;
    skos:prefLabel "Pref label"@en .

locn:geographicName a owl:DatatypeProperty ;
    skos:definition "A textual description for a Location. (dct:Location)"@en ;
    skos:prefLabel "Geographic name"@en .

foaf:homepage a owl:DatatypeProperty ;
    skos:prefLabel "Homepage"@en .

foaf:mbox a owl:DatatypeProperty ;
    skos:prefLabel "Mbox"@en .

foaf:name a owl:DatatypeProperty ;
    skos:definition "The complete name of the Candidate as one string. (rmo:Candidate)"@en ;
    skos:prefLabel "Name"@en .

rmo:Credential a owl:Class ;
    rdfs:isDefinedBy rmo:tech ;
    skos:definition "An academic or professional qualification obtained by a candidate, such as degrees or certifications."@en ;
    skos:prefLabel "Credential"@en .

rmo:tech a owl:Ontology ;
    rdfs:label "Core Recruitment Match Vocabulary - core"@en ;
    dcterms:created "2024-07-01"^^xsd:date ;
    dcterms:description "The Recruitment Match Ontology core describes the concepts and properties representing the Recruitment domain. The provision of these semantics offers the basis for a common understanding of the domain for all stakeholders ensuring the quality of data exchange and transparency. The ontology restrictions are published in a separate artefact."@en ;
    dcterms:issued "2024-07-26"^^xsd:date ;
    dcterms:license "© Meaningfy, 2024. Unless otherwise noted, the reuse of the Ontology is authorised under the Meaningfy  CC-BY 4.0." ;
    dcterms:publisher "https://meaningfy.ws/" ;
    dcterms:title "RMO Ontology  - core"@en ;
    vann:preferredNamespacePrefix "rmo" ;
    vann:preferredNamespaceUri "http://index.dev/ontology/rmo#" ;
    rdfs:comment "This version is automatically generated from poc_CM.xml on 2024-07-26" ;
    rdfs:seeAlso <https://docs.ted.europa.eu/home/index.html>,
        <https://github.com/OP-TED/ePO/releases>,
        <https://joinup.ec.europa.eu/collection/eprocurement/solution/eprocurement-ontology/about>,
        <https://op.europa.eu/en/web/eu-vocabularies/e-procurement> ;
    owl:imports <http://data.europa.eu/esco/model>,
        cccev:,
        <http://data.europa.eu/nuts>,
        <http://lexvo.org/ontology>,
        <http://publications.europa.eu/ontology/euvoc>,
        at-voc:,
        dcterms:,
        <http://www.lexinfo.net/ontology/2.0/lexinfo>,
        <http://www.opengis.net/ont/geosparql>,
        <http://www.opengis.net/ont/sf>,
        <http://www.w3.org/2003/01/geo/wgs84_pos>,
        <http://www.w3.org/2004/02/skos/core>,
        <http://www.w3.org/2006/time>,
        <http://www.w3.org/2006/vcard/ns>,
        <http://www.w3.org/2008/05/skos-xl>,
        <http://www.w3.org/ns/adms>,
        <http://www.w3.org/ns/locn>,
        org:,
        <http://www.w3.org/ns/person>,
        foaf:,
        <https://data.europa.eu/m8g/>,
        <ttp://publications.europa.eu/ontology/authority/> ;
    owl:incompatibleWith "3.1.0" ;
    owl:priorVersion "http://index.dev/ontology/rmo#tech-3.1.0" ;
    owl:versionIRI rmo:tech-4.0.0 ;
    owl:versionInfo "4.0.0" .

