<?xml version="1.0" encoding="UTF-8"?>
<rdf:RDF xmlns="http://index.dev/ontology/rmo#"
         xmlns:adms="http://www.w3.org/ns/adms#"
         xmlns:cccev="http://data.europa.eu/m8g/"
         xmlns:cpov="http://data.europa.eu/m8g/"
         xmlns:cpsv="http://data.europa.eu/m8g/"
         xmlns:cpv="http://data.europa.eu/m8g/"
         xmlns:cv="http://data.europa.eu/m8g/"
         xmlns:dc="http://purl.org/dc/elements/1.1/"
         xmlns:dct="http://purl.org/dc/terms/"
         xmlns:dul="http://www.ontologydesignpatterns.org/ont/dul/DUL.owl#"
         xmlns:esco="http://data.europa.eu/esco/model#"
         xmlns:foaf="http://xmlns.com/foaf/0.1/"
         xmlns:geosparql="http://www.opengis.net/ont/geosparql#"
         xmlns:lexinfo="http://www.lexinfo.net/ontology/2.0/lexinfo#"
         xmlns:lexvo="http://lexvo.org/ontology#"
         xmlns:locn="http://www.w3.org/ns/locn#"
         xmlns:org="http://www.w3.org/ns/org#"
         xmlns:owl="http://www.w3.org/2002/07/owl#"
         xmlns:person="http://www.w3.org/ns/person#"
         xmlns:rdf="http://www.w3.org/1999/02/22-rdf-syntax-ns#"
         xmlns:rdfs="http://www.w3.org/2000/01/rdf-schema#"
         xmlns:rmo="http://index.dev/ontology/rmo#"
         xmlns:sf="http://www.opengis.net/ont/sf#"
         xmlns:skos="http://www.w3.org/2004/02/skos/core#"
         xmlns:skosxl="http://www.w3.org/2008/05/skos-xl#"
         xmlns:time="http://www.w3.org/2006/time#"
         xmlns:vann="http://purl.org/vocab/vann/"
         xmlns:vcard="http://www.w3.org/2006/vcard/ns#"
         xmlns:wgs="http://www.w3.org/2003/01/geo/wgs84_pos#"
         xmlns:xsd="http://www.w3.org/2001/XMLSchema#">
   <owl:Ontology rdf:about="http://index.dev/ontology/rmo#tech">
      <owl:imports rdf:resource="http://xmlns.com/foaf/0.1/"/>
      <owl:imports rdf:resource="http://purl.org/dc/terms/"/>
      <owl:imports rdf:resource="http://www.w3.org/ns/org#"/>
      <owl:imports rdf:resource="http://www.w3.org/2004/02/skos/core"/>
      <owl:imports rdf:resource="http://www.w3.org/2006/time"/>
      <owl:imports rdf:resource="http://www.w3.org/ns/locn"/>
      <owl:imports rdf:resource="https://data.europa.eu/m8g/"/>
      <owl:imports rdf:resource="http://data.europa.eu/m8g/"/>
      <owl:imports rdf:resource="http://data.europa.eu/m8g/"/>
      <owl:imports rdf:resource="http://data.europa.eu/m8g/"/>
      <owl:imports rdf:resource="https://data.europa.eu/m8g/"/>
      <owl:imports rdf:resource="http://www.opengis.net/ont/geosparql"/>
      <owl:imports rdf:resource="http://www.w3.org/ns/person"/>
      <owl:imports rdf:resource="http://www.w3.org/ns/adms"/>
      <owl:imports rdf:resource="http://www.w3.org/2003/01/geo/wgs84_pos"/>
      <owl:imports rdf:resource="http://publications.europa.eu/ontology/euvoc"/>
      <owl:imports rdf:resource="http://lexvo.org/ontology"/>
      <owl:imports rdf:resource="http://www.w3.org/2008/05/skos-xl"/>
      <owl:imports rdf:resource="http://www.lexinfo.net/ontology/2.0/lexinfo"/>
      <owl:imports rdf:resource="http://www.w3.org/2006/vcard/ns"/>
      <owl:imports rdf:resource="http://www.opengis.net/ont/sf"/>
      <owl:imports rdf:resource="http://data.europa.eu/esco/model"/>
      <dct:title xml:lang="en">Recruitment Match Ontology (RMO) - core</dct:title>
      <rdfs:label xml:lang="en">Core Recruitment Match Vocabulary - core</rdfs:label>
      <dct:description xml:lang="en">The Recruitment Match Ontology core describes the concepts and properties representing the Recruitment domain. The provision of these semantics offers the basis for a common understanding of the domain for all stakeholders ensuring the quality of data exchange and transparency. The ontology restrictions are published in a separate artefact.</dct:description>
      <dct:publisher>https://meaningfy.ws/</dct:publisher>
      <rdfs:comment>This version is automatically generated from poc_CM.xml on 2024-07-28</rdfs:comment>
      <rdfs:seeAlso rdf:resource="https://github.com/meaningfy-ws/rmo-ontology"/>
      <dct:issued rdf:datatype="http://www.w3.org/2001/XMLSchema#date">2024-07-28</dct:issued>
      <dct:created rdf:datatype="http://www.w3.org/2001/XMLSchema#date">2024-07-01</dct:created>
      <owl:versionInfo>1.0.0</owl:versionInfo>
      <owl:incompatibleWith>none</owl:incompatibleWith>
      <owl:versionIRI rdf:resource="http://index.dev/ontology/rmo#tech-1.0.0"/>
      <owl:priorVersion>http://index.dev/ontology/rmo#tech-none</owl:priorVersion>
      <vann:preferredNamespaceUri>http://index.dev/ontology/rmo#</vann:preferredNamespaceUri>
      <vann:preferredNamespacePrefix>rmo</vann:preferredNamespacePrefix>
      <dct:license>Â© Meaningfy, 2024. Unless otherwise noted, the reuse of the Ontology is authorised under the Meaningfy  CC-BY 4.0.</dct:license>
   </owl:Ontology>
   <owl:Class rdf:about="http://purl.org/dc/terms/Location"/>
   <rdf:Description rdf:about="http://purl.org/dc/terms/Location">
      <skos:prefLabel xml:lang="en">Location</skos:prefLabel>
   </rdf:Description>
   <rdf:Description rdf:about="http://purl.org/dc/terms/Location">
      <skos:definition xml:lang="en">A geographic area or place characterized by its physical coordinates and corresponding time zone.</skos:definition>
   </rdf:Description>
   <owl:Class rdf:about="http://index.dev/ontology/rmo#Benefits"/>
   <rdf:Description rdf:about="http://index.dev/ontology/rmo#Benefits">
      <skos:prefLabel xml:lang="en">Benefits</skos:prefLabel>
   </rdf:Description>
   <rdf:Description rdf:about="http://index.dev/ontology/rmo#Benefits">
      <skos:definition xml:lang="en">Additional advantages provided to employees beyond their salary, such as health insurance or retirement plans.</skos:definition>
   </rdf:Description>
   <rdf:Description rdf:about="http://index.dev/ontology/rmo#Benefits">
      <rdfs:isDefinedBy rdf:resource="http://index.dev/ontology/rmo#tech"/>
   </rdf:Description>
   <owl:Class rdf:about="http://index.dev/ontology/rmo#Candidate"/>
   <rdf:Description rdf:about="http://index.dev/ontology/rmo#Candidate">
      <skos:prefLabel xml:lang="en">Candidate</skos:prefLabel>
   </rdf:Description>
   <rdf:Description rdf:about="http://index.dev/ontology/rmo#Candidate">
      <skos:definition xml:lang="en">An individual who uses the system to find job opportunities.</skos:definition>
   </rdf:Description>
   <rdf:Description rdf:about="http://index.dev/ontology/rmo#Candidate">
      <rdfs:isDefinedBy rdf:resource="http://index.dev/ontology/rmo#tech"/>
   </rdf:Description>
   <owl:Class rdf:about="http://index.dev/ontology/rmo#CandidateProfile"/>
   <rdf:Description rdf:about="http://index.dev/ontology/rmo#CandidateProfile">
      <skos:prefLabel xml:lang="en">Candidate profile</skos:prefLabel>
   </rdf:Description>
   <rdf:Description rdf:about="http://index.dev/ontology/rmo#CandidateProfile">
      <skos:definition xml:lang="en">Represents the detailed profile of a Candidate, including credentials, skills experience, and location.</skos:definition>
   </rdf:Description>
   <rdf:Description rdf:about="http://index.dev/ontology/rmo#CandidateProfile">
      <rdfs:isDefinedBy rdf:resource="http://index.dev/ontology/rmo#tech"/>
   </rdf:Description>
   <owl:Class rdf:about="http://index.dev/ontology/rmo#Certification"/>
   <rdf:Description rdf:about="http://index.dev/ontology/rmo#Certification">
      <skos:prefLabel xml:lang="en">Certification</skos:prefLabel>
   </rdf:Description>
   <rdf:Description rdf:about="http://index.dev/ontology/rmo#Certification">
      <skos:definition xml:lang="en">The official recognition of a candidate's expertise or proficiency in a specific domain, typically obtained through examination or evaluation by a professional body.</skos:definition>
   </rdf:Description>
   <rdf:Description rdf:about="http://index.dev/ontology/rmo#Certification">
      <rdfs:isDefinedBy rdf:resource="http://index.dev/ontology/rmo#tech"/>
   </rdf:Description>
   <owl:Class rdf:about="http://index.dev/ontology/rmo#Company"/>
   <rdf:Description rdf:about="http://index.dev/ontology/rmo#Company">
      <skos:prefLabel xml:lang="en">Company</skos:prefLabel>
   </rdf:Description>
   <rdf:Description rdf:about="http://index.dev/ontology/rmo#Company">
      <skos:definition xml:lang="en">An organization or business entity that employs individuals.</skos:definition>
   </rdf:Description>
   <rdf:Description rdf:about="http://index.dev/ontology/rmo#Company">
      <rdfs:isDefinedBy rdf:resource="http://index.dev/ontology/rmo#tech"/>
   </rdf:Description>
   <owl:Class rdf:about="http://index.dev/ontology/rmo#Credential"/>
   <rdf:Description rdf:about="http://index.dev/ontology/rmo#Credential">
      <skos:prefLabel xml:lang="en">Credential</skos:prefLabel>
   </rdf:Description>
   <rdf:Description rdf:about="http://index.dev/ontology/rmo#Credential">
      <skos:definition xml:lang="en">An academic or professional qualification obtained by a candidate, such as degrees or certifications.</skos:definition>
   </rdf:Description>
   <rdf:Description rdf:about="http://index.dev/ontology/rmo#Credential">
      <rdfs:isDefinedBy rdf:resource="http://index.dev/ontology/rmo#tech"/>
   </rdf:Description>
   <owl:Class rdf:about="http://index.dev/ontology/rmo#Education"/>
   <rdf:Description rdf:about="http://index.dev/ontology/rmo#Education">
      <skos:prefLabel xml:lang="en">Education</skos:prefLabel>
   </rdf:Description>
   <rdf:Description rdf:about="http://index.dev/ontology/rmo#Education">
      <skos:definition xml:lang="en">The academic qualifications of a Candidate.</skos:definition>
   </rdf:Description>
   <rdf:Description rdf:about="http://index.dev/ontology/rmo#Education">
      <rdfs:isDefinedBy rdf:resource="http://index.dev/ontology/rmo#tech"/>
   </rdf:Description>
   <owl:Class rdf:about="http://index.dev/ontology/rmo#Experience"/>
   <rdf:Description rdf:about="http://index.dev/ontology/rmo#Experience">
      <skos:prefLabel xml:lang="en">Experience</skos:prefLabel>
   </rdf:Description>
   <rdf:Description rdf:about="http://index.dev/ontology/rmo#Experience">
      <skos:definition xml:lang="en">Represents the practical knowledge and proficiency gained by a candidate through previous work engagements, projects, or hands-on activities.</skos:definition>
   </rdf:Description>
   <rdf:Description rdf:about="http://index.dev/ontology/rmo#Experience">
      <rdfs:isDefinedBy rdf:resource="http://index.dev/ontology/rmo#tech"/>
   </rdf:Description>
   <owl:Class rdf:about="http://index.dev/ontology/rmo#JobDescription"/>
   <rdf:Description rdf:about="http://index.dev/ontology/rmo#JobDescription">
      <skos:prefLabel xml:lang="en">Job description</skos:prefLabel>
   </rdf:Description>
   <rdf:Description rdf:about="http://index.dev/ontology/rmo#JobDescription">
      <skos:definition xml:lang="en">A job opening posted by a company, including job details and requirements.</skos:definition>
   </rdf:Description>
   <rdf:Description rdf:about="http://index.dev/ontology/rmo#JobDescription">
      <rdfs:isDefinedBy rdf:resource="http://index.dev/ontology/rmo#tech"/>
   </rdf:Description>
   <owl:Class rdf:about="http://index.dev/ontology/rmo#Qualification"/>
   <rdf:Description rdf:about="http://index.dev/ontology/rmo#Qualification">
      <skos:prefLabel xml:lang="en">Qualification</skos:prefLabel>
   </rdf:Description>
   <rdf:Description rdf:about="http://index.dev/ontology/rmo#Qualification">
      <skos:definition xml:lang="en">Qualifications are the formal outcome of an assessment and validation process by a competent body determining that an individual has achieved learning outcomes to given standards.</skos:definition>
   </rdf:Description>
   <rdf:Description rdf:about="http://index.dev/ontology/rmo#Qualification">
      <rdfs:isDefinedBy rdf:resource="http://index.dev/ontology/rmo#tech"/>
   </rdf:Description>
   <owl:Class rdf:about="http://index.dev/ontology/rmo#Role"/>
   <rdf:Description rdf:about="http://index.dev/ontology/rmo#Role">
      <skos:prefLabel xml:lang="en">Role</skos:prefLabel>
   </rdf:Description>
   <rdf:Description rdf:about="http://index.dev/ontology/rmo#Role">
      <skos:definition xml:lang="en">Represents the specific job occupations, positions, or professions for which candidates may be qualified or seeking employment opportunities.</skos:definition>
   </rdf:Description>
   <rdf:Description rdf:about="http://index.dev/ontology/rmo#Role">
      <rdfs:isDefinedBy rdf:resource="http://index.dev/ontology/rmo#tech"/>
   </rdf:Description>
   <owl:Class rdf:about="http://index.dev/ontology/rmo#Skill"/>
   <rdf:Description rdf:about="http://index.dev/ontology/rmo#Skill">
      <skos:prefLabel xml:lang="en">Skill</skos:prefLabel>
   </rdf:Description>
   <rdf:Description rdf:about="http://index.dev/ontology/rmo#Skill">
      <skos:definition xml:lang="en">A specific capability or proficiency possessed by a candidate, often acquired through training, practice, or experience.</skos:definition>
   </rdf:Description>
   <rdf:Description rdf:about="http://index.dev/ontology/rmo#Skill">
      <rdfs:isDefinedBy rdf:resource="http://index.dev/ontology/rmo#tech"/>
   </rdf:Description>
   <owl:Class rdf:about="http://index.dev/ontology/rmo#TypeOfEngagement"/>
   <rdf:Description rdf:about="http://index.dev/ontology/rmo#TypeOfEngagement">
      <skos:prefLabel xml:lang="en">Type of engagement</skos:prefLabel>
   </rdf:Description>
   <rdf:Description rdf:about="http://index.dev/ontology/rmo#TypeOfEngagement">
      <skos:definition xml:lang="en">Represents various arrangements under which individuals are employed, such as part-time, full-time, or contractual roles.</skos:definition>
   </rdf:Description>
   <rdf:Description rdf:about="http://index.dev/ontology/rmo#TypeOfEngagement">
      <rdfs:isDefinedBy rdf:resource="http://index.dev/ontology/rmo#tech"/>
   </rdf:Description>
   <skos:ConceptScheme rdf:about="http://data.europa.eu/esco/model#Occupation"/>
   <rdf:Description rdf:about="http://data.europa.eu/esco/model#Occupation">
      <skos:prefLabel xml:lang="en">Occupation</skos:prefLabel>
   </rdf:Description>
   <skos:ConceptScheme rdf:about="http://data.europa.eu/esco/model#Qualification"/>
   <rdf:Description rdf:about="http://data.europa.eu/esco/model#Qualification">
      <skos:prefLabel xml:lang="en">Qualification</skos:prefLabel>
   </rdf:Description>
   <skos:ConceptScheme rdf:about="http://data.europa.eu/esco/model#Skill"/>
   <rdf:Description rdf:about="http://data.europa.eu/esco/model#Skill">
      <skos:prefLabel xml:lang="en">Skill</skos:prefLabel>
   </rdf:Description>
   <owl:NamedIndividual rdf:about="http://data.europa.eu/esco/model#Occupation">
      <rdf:type rdf:resource="http://www.w3.org/2004/02/skos/core#ConceptScheme"/>
   </owl:NamedIndividual>
   <owl:NamedIndividual rdf:about="http://data.europa.eu/esco/model#Qualification">
      <rdf:type rdf:resource="http://www.w3.org/2004/02/skos/core#ConceptScheme"/>
   </owl:NamedIndividual>
   <owl:NamedIndividual rdf:about="http://data.europa.eu/esco/model#Skill">
      <rdf:type rdf:resource="http://www.w3.org/2004/02/skos/core#ConceptScheme"/>
   </owl:NamedIndividual>
   <owl:Class rdf:about="http://index.dev/ontology/rmo#Certification">
      <rdfs:subClassOf rdf:resource="http://index.dev/ontology/rmo#Credential"/>
   </owl:Class>
   <owl:Class rdf:about="http://index.dev/ontology/rmo#Education">
      <rdfs:subClassOf rdf:resource="http://index.dev/ontology/rmo#Credential"/>
   </owl:Class>
   <owl:Class rdf:about="http://index.dev/ontology/rmo#Qualification">
      <rdfs:subClassOf rdf:resource="http://www.w3.org/2004/02/skos/core#Concept"/>
   </owl:Class>
   <owl:Class rdf:about="http://index.dev/ontology/rmo#Role">
      <rdfs:subClassOf rdf:resource="http://www.w3.org/2004/02/skos/core#Concept"/>
   </owl:Class>
   <owl:Class rdf:about="http://index.dev/ontology/rmo#Skill">
      <rdfs:subClassOf rdf:resource="http://www.w3.org/2004/02/skos/core#Concept"/>
   </owl:Class>
   <owl:ObjectProperty rdf:about="http://index.dev/ontology/rmo#specifiesLocation"/>
   <rdf:Description rdf:about="http://index.dev/ontology/rmo#specifiesLocation">
      <skos:prefLabel xml:lang="en">Specifies location</skos:prefLabel>
   </rdf:Description>
   <rdf:Description rdf:about="http://index.dev/ontology/rmo#specifiesLocation">
      <skos:definition xml:lang="en">Specifies the geographical location and time zone relevant to job description. (rmo:JobDescription -&gt; dct:Location (+rmo:specifiesLocation))</skos:definition>
   </rdf:Description>
   <rdf:Description rdf:about="http://index.dev/ontology/rmo#specifiesLocation">
      <rdfs:isDefinedBy rdf:resource="http://index.dev/ontology/rmo#tech"/>
   </rdf:Description>
   <owl:ObjectProperty rdf:about="http://index.dev/ontology/rmo#hasLocation"/>
   <rdf:Description rdf:about="http://index.dev/ontology/rmo#hasLocation">
      <skos:prefLabel xml:lang="en">Has location</skos:prefLabel>
   </rdf:Description>
   <rdf:Description rdf:about="http://index.dev/ontology/rmo#hasLocation">
      <skos:definition xml:lang="en">Specifies the geographical location and time zone relevant to candidate profile. (rmo:Company -&gt; dct:Location (+rmo:hasLocation)) Specifies the geographical location and timezone relevant to CandidateProfile. (rmo:CandidateProfile -&gt; dct:Location (+rmo:hasLocation))</skos:definition>
   </rdf:Description>
   <rdf:Description rdf:about="http://index.dev/ontology/rmo#hasLocation">
      <rdfs:isDefinedBy rdf:resource="http://index.dev/ontology/rmo#tech"/>
   </rdf:Description>
   <owl:ObjectProperty rdf:about="http://index.dev/ontology/rmo#hasBenefits"/>
   <rdf:Description rdf:about="http://index.dev/ontology/rmo#hasBenefits">
      <skos:prefLabel xml:lang="en">Has benefits</skos:prefLabel>
   </rdf:Description>
   <rdf:Description rdf:about="http://index.dev/ontology/rmo#hasBenefits">
      <skos:definition xml:lang="en">Indicates the benefits associated with a specific type of job engagement. (rmo:TypeOfEngagement -&gt; rmo:Benefits (+rmo:hasBenefits))</skos:definition>
   </rdf:Description>
   <rdf:Description rdf:about="http://index.dev/ontology/rmo#hasBenefits">
      <rdfs:isDefinedBy rdf:resource="http://index.dev/ontology/rmo#tech"/>
   </rdf:Description>
   <owl:ObjectProperty rdf:about="http://index.dev/ontology/rmo#hasProfile"/>
   <rdf:Description rdf:about="http://index.dev/ontology/rmo#hasProfile">
      <skos:prefLabel xml:lang="en">Has profile</skos:prefLabel>
   </rdf:Description>
   <rdf:Description rdf:about="http://index.dev/ontology/rmo#hasProfile">
      <skos:definition xml:lang="en">Indicates the candidate profile of a specific Candidate. (rmo:Candidate -&gt; rmo:CandidateProfile (+rmo:hasProfile))</skos:definition>
   </rdf:Description>
   <rdf:Description rdf:about="http://index.dev/ontology/rmo#hasProfile">
      <rdfs:isDefinedBy rdf:resource="http://index.dev/ontology/rmo#tech"/>
   </rdf:Description>
   <owl:ObjectProperty rdf:about="http://index.dev/ontology/rmo#hasExperience"/>
   <rdf:Description rdf:about="http://index.dev/ontology/rmo#hasExperience">
      <skos:prefLabel xml:lang="en">Has experience</skos:prefLabel>
   </rdf:Description>
   <rdf:Description rdf:about="http://index.dev/ontology/rmo#hasExperience">
      <skos:definition xml:lang="en">Represents the work experience details of a candidate profile. (rmo:CandidateProfile -&gt; rmo:Experience (+rmo:hasExperience))</skos:definition>
   </rdf:Description>
   <rdf:Description rdf:about="http://index.dev/ontology/rmo#hasExperience">
      <rdfs:isDefinedBy rdf:resource="http://index.dev/ontology/rmo#tech"/>
   </rdf:Description>
   <owl:ObjectProperty rdf:about="http://index.dev/ontology/rmo#receivesJobDesciption"/>
   <rdf:Description rdf:about="http://index.dev/ontology/rmo#receivesJobDesciption">
      <skos:prefLabel xml:lang="en">Receives job desciption</skos:prefLabel>
   </rdf:Description>
   <rdf:Description rdf:about="http://index.dev/ontology/rmo#receivesJobDesciption">
      <skos:definition xml:lang="en">Indicates that a candidate profile receives a job description from the system. (rmo:CandidateProfile -&gt; rmo:JobDescription (+rmo:receivesJobDesciption))</skos:definition>
   </rdf:Description>
   <rdf:Description rdf:about="http://index.dev/ontology/rmo#receivesJobDesciption">
      <rdfs:isDefinedBy rdf:resource="http://index.dev/ontology/rmo#tech"/>
   </rdf:Description>
   <owl:ObjectProperty rdf:about="http://index.dev/ontology/rmo#targetOccupation"/>
   <rdf:Description rdf:about="http://index.dev/ontology/rmo#targetOccupation">
      <skos:prefLabel xml:lang="en">Target occupation</skos:prefLabel>
   </rdf:Description>
   <rdf:Description rdf:about="http://index.dev/ontology/rmo#targetOccupation">
      <skos:definition xml:lang="en">Indicates the job roles or occupations that a candidate profile is interested in or qualified for. (rmo:CandidateProfile -&gt; rmo:Role (+rmo:targetOccupation))</skos:definition>
   </rdf:Description>
   <rdf:Description rdf:about="http://index.dev/ontology/rmo#targetOccupation">
      <rdfs:isDefinedBy rdf:resource="http://index.dev/ontology/rmo#tech"/>
   </rdf:Description>
   <owl:ObjectProperty rdf:about="http://index.dev/ontology/rmo#hasQualification"/>
   <rdf:Description rdf:about="http://index.dev/ontology/rmo#hasQualification">
      <skos:prefLabel xml:lang="en">Has qualification</skos:prefLabel>
   </rdf:Description>
   <rdf:Description rdf:about="http://index.dev/ontology/rmo#hasQualification">
      <rdfs:isDefinedBy rdf:resource="http://index.dev/ontology/rmo#tech"/>
   </rdf:Description>
   <owl:ObjectProperty rdf:about="http://index.dev/ontology/rmo#hasCredential"/>
   <rdf:Description rdf:about="http://index.dev/ontology/rmo#hasCredential">
      <skos:prefLabel xml:lang="en">Has credential</skos:prefLabel>
   </rdf:Description>
   <rdf:Description rdf:about="http://index.dev/ontology/rmo#hasCredential">
      <skos:definition xml:lang="en">Academic qualifications and professional certifications obtained by a candidate. (rmo:CandidateProfile -&gt; rmo:Credential (+rmo:hasCredential))</skos:definition>
   </rdf:Description>
   <rdf:Description rdf:about="http://index.dev/ontology/rmo#hasCredential">
      <rdfs:isDefinedBy rdf:resource="http://index.dev/ontology/rmo#tech"/>
   </rdf:Description>
   <owl:ObjectProperty rdf:about="http://index.dev/ontology/rmo#hasSkills"/>
   <rdf:Description rdf:about="http://index.dev/ontology/rmo#hasSkills">
      <skos:prefLabel xml:lang="en">Has skills</skos:prefLabel>
   </rdf:Description>
   <rdf:Description rdf:about="http://index.dev/ontology/rmo#hasSkills">
      <skos:definition xml:lang="en">Indicates that a candidate profile possesses a specific skill. (rmo:CandidateProfile -&gt; rmo:Skill (+rmo:hasSkills))</skos:definition>
   </rdf:Description>
   <rdf:Description rdf:about="http://index.dev/ontology/rmo#hasSkills">
      <rdfs:isDefinedBy rdf:resource="http://index.dev/ontology/rmo#tech"/>
   </rdf:Description>
   <owl:ObjectProperty rdf:about="http://index.dev/ontology/rmo#posts"/>
   <rdf:Description rdf:about="http://index.dev/ontology/rmo#posts">
      <skos:prefLabel xml:lang="en">Posts</skos:prefLabel>
   </rdf:Description>
   <rdf:Description rdf:about="http://index.dev/ontology/rmo#posts">
      <skos:definition xml:lang="en">Indicates that a Company publishes a job description. (rmo:Company -&gt; rmo:JobDescription (+rmo:posts))</skos:definition>
   </rdf:Description>
   <rdf:Description rdf:about="http://index.dev/ontology/rmo#posts">
      <rdfs:isDefinedBy rdf:resource="http://index.dev/ontology/rmo#tech"/>
   </rdf:Description>
   <owl:ObjectProperty rdf:about="http://index.dev/ontology/rmo#requiresCredential"/>
   <rdf:Description rdf:about="http://index.dev/ontology/rmo#requiresCredential">
      <skos:prefLabel xml:lang="en">Requires credential</skos:prefLabel>
   </rdf:Description>
   <rdf:Description rdf:about="http://index.dev/ontology/rmo#requiresCredential">
      <skos:definition xml:lang="en">Indicates that a job description may require one or more Academic qualifications and/or professional certifications. (rmo:JobDescription -&gt; rmo:Credential (+rmo:requiresCredential))</skos:definition>
   </rdf:Description>
   <rdf:Description rdf:about="http://index.dev/ontology/rmo#requiresCredential">
      <rdfs:isDefinedBy rdf:resource="http://index.dev/ontology/rmo#tech"/>
   </rdf:Description>
   <owl:ObjectProperty rdf:about="http://index.dev/ontology/rmo#isRelatedTo"/>
   <rdf:Description rdf:about="http://index.dev/ontology/rmo#isRelatedTo">
      <skos:prefLabel xml:lang="en">Is related to</skos:prefLabel>
   </rdf:Description>
   <rdf:Description rdf:about="http://index.dev/ontology/rmo#isRelatedTo">
      <skos:definition xml:lang="en">Indicates that a specific resource is associated with a particular other resource. (rmo:Experience -&gt; rmo:Role (+rmo:isRelatedTo)) Indicates that a specific resource is associated with a particular other resource. (rmo:Experience -&gt; rmo:Qualification (+rmo:isRelatedTo))</skos:definition>
   </rdf:Description>
   <rdf:Description rdf:about="http://index.dev/ontology/rmo#isRelatedTo">
      <rdfs:isDefinedBy rdf:resource="http://index.dev/ontology/rmo#tech"/>
   </rdf:Description>
   <owl:ObjectProperty rdf:about="http://index.dev/ontology/rmo#hasSkillUsed"/>
   <rdf:Description rdf:about="http://index.dev/ontology/rmo#hasSkillUsed">
      <skos:prefLabel xml:lang="en">Has skill used</skos:prefLabel>
   </rdf:Description>
   <rdf:Description rdf:about="http://index.dev/ontology/rmo#hasSkillUsed">
      <skos:definition xml:lang="en">Indicates that a specific skill was utilized in a particular experience. (rmo:Experience -&gt; rmo:Skill (+rmo:hasSkillUsed))</skos:definition>
   </rdf:Description>
   <rdf:Description rdf:about="http://index.dev/ontology/rmo#hasSkillUsed">
      <rdfs:isDefinedBy rdf:resource="http://index.dev/ontology/rmo#tech"/>
   </rdf:Description>
   <owl:ObjectProperty rdf:about="http://index.dev/ontology/rmo#requiresExperience"/>
   <rdf:Description rdf:about="http://index.dev/ontology/rmo#requiresExperience">
      <skos:prefLabel xml:lang="en">Requires experience</skos:prefLabel>
   </rdf:Description>
   <rdf:Description rdf:about="http://index.dev/ontology/rmo#requiresExperience">
      <skos:definition xml:lang="en">Specifies the type and level of experience required for a job description. (rmo:JobDescription -&gt; rmo:Experience (+rmo:requiresExperience))</skos:definition>
   </rdf:Description>
   <rdf:Description rdf:about="http://index.dev/ontology/rmo#requiresExperience">
      <rdfs:isDefinedBy rdf:resource="http://index.dev/ontology/rmo#tech"/>
   </rdf:Description>
   <owl:ObjectProperty rdf:about="http://index.dev/ontology/rmo#hasEngagement"/>
   <rdf:Description rdf:about="http://index.dev/ontology/rmo#hasEngagement">
      <skos:prefLabel xml:lang="en">Has engagement</skos:prefLabel>
   </rdf:Description>
   <rdf:Description rdf:about="http://index.dev/ontology/rmo#hasEngagement">
      <skos:definition xml:lang="en">Indicates what type of engagement a specific job description entails. (rmo:JobDescription -&gt; rmo:TypeOfEngagement (+rmo:hasEngagement))</skos:definition>
   </rdf:Description>
   <rdf:Description rdf:about="http://index.dev/ontology/rmo#hasEngagement">
      <rdfs:isDefinedBy rdf:resource="http://index.dev/ontology/rmo#tech"/>
   </rdf:Description>
   <owl:ObjectProperty rdf:about="http://index.dev/ontology/rmo#requiresQualification"/>
   <rdf:Description rdf:about="http://index.dev/ontology/rmo#requiresQualification">
      <skos:prefLabel xml:lang="en">Requires qualification</skos:prefLabel>
   </rdf:Description>
   <rdf:Description rdf:about="http://index.dev/ontology/rmo#requiresQualification">
      <skos:definition xml:lang="en">Specifies the qualifications required for a job description. (rmo:JobDescription -&gt; rmo:Qualification (+rmo:requiresQualification))</skos:definition>
   </rdf:Description>
   <rdf:Description rdf:about="http://index.dev/ontology/rmo#requiresQualification">
      <rdfs:isDefinedBy rdf:resource="http://index.dev/ontology/rmo#tech"/>
   </rdf:Description>
   <owl:ObjectProperty rdf:about="http://index.dev/ontology/rmo#offersPosition"/>
   <rdf:Description rdf:about="http://index.dev/ontology/rmo#offersPosition">
      <skos:prefLabel xml:lang="en">Offers position</skos:prefLabel>
   </rdf:Description>
   <rdf:Description rdf:about="http://index.dev/ontology/rmo#offersPosition">
      <skos:definition xml:lang="en">Indicates the job position offered by a job description. (rmo:JobDescription -&gt; rmo:Role (+rmo:offersPosition))</skos:definition>
   </rdf:Description>
   <rdf:Description rdf:about="http://index.dev/ontology/rmo#offersPosition">
      <rdfs:isDefinedBy rdf:resource="http://index.dev/ontology/rmo#tech"/>
   </rdf:Description>
   <owl:ObjectProperty rdf:about="http://index.dev/ontology/rmo#requiresSkill"/>
   <rdf:Description rdf:about="http://index.dev/ontology/rmo#requiresSkill">
      <skos:prefLabel xml:lang="en">Requires skill</skos:prefLabel>
   </rdf:Description>
   <rdf:Description rdf:about="http://index.dev/ontology/rmo#requiresSkill">
      <skos:definition xml:lang="en">Specifies the skills that are necessary for a job description. (rmo:JobDescription -&gt; rmo:Skill (+rmo:requiresSkill))</skos:definition>
   </rdf:Description>
   <rdf:Description rdf:about="http://index.dev/ontology/rmo#requiresSkill">
      <rdfs:isDefinedBy rdf:resource="http://index.dev/ontology/rmo#tech"/>
   </rdf:Description>
   <owl:ObjectProperty rdf:about="http://www.w3.org/2004/02/skos/core#inScheme"/>
   <rdf:Description rdf:about="http://www.w3.org/2004/02/skos/core#inScheme">
      <skos:prefLabel xml:lang="en">In scheme</skos:prefLabel>
   </rdf:Description>
   <rdf:Description rdf:about="http://www.w3.org/2004/02/skos/core#inScheme">
      <skos:definition xml:lang="en">A Concept Scheme in which the Concept is included. A Concept may be a member of more than one concept scheme. (rmo:Qualification -&gt; esco:Qualification (+skos:inScheme)) A Concept Scheme in which the Concept is included. A Concept may be a member of more than one concept scheme. (rmo:Role -&gt; esco:Occupation (+skos:inScheme)) A Concept Scheme in which the Concept is included. A Concept may be a member of more than one concept scheme. (rmo:Skill -&gt; esco:Skill (+skos:inScheme))</skos:definition>
   </rdf:Description>
   <owl:ObjectProperty rdf:about="http://index.dev/ontology/rmo#optionalFor"/>
   <rdf:Description rdf:about="http://index.dev/ontology/rmo#optionalFor">
      <skos:prefLabel xml:lang="en">Optional for</skos:prefLabel>
   </rdf:Description>
   <rdf:Description rdf:about="http://index.dev/ontology/rmo#optionalFor">
      <skos:definition xml:lang="en">Indicates that a particular resource or characteristic is optional or non-compulsory for a specific entity or concept within the ontology. (rmo:Skill -&gt; rmo:Role (+rmo:optionalFor))</skos:definition>
   </rdf:Description>
   <rdf:Description rdf:about="http://index.dev/ontology/rmo#optionalFor">
      <rdfs:isDefinedBy rdf:resource="http://index.dev/ontology/rmo#tech"/>
   </rdf:Description>
   <owl:ObjectProperty rdf:about="http://index.dev/ontology/rmo#essentialFor"/>
   <rdf:Description rdf:about="http://index.dev/ontology/rmo#essentialFor">
      <skos:prefLabel xml:lang="en">Essential for</skos:prefLabel>
   </rdf:Description>
   <rdf:Description rdf:about="http://index.dev/ontology/rmo#essentialFor">
      <skos:definition xml:lang="en">Indicates that a particular resource or characteristic is necessary or crucial for a specific entity or concept within the ontology in order to fulfill its intended purpose. (rmo:Skill -&gt; rmo:Role (+rmo:essentialFor))</skos:definition>
   </rdf:Description>
   <rdf:Description rdf:about="http://index.dev/ontology/rmo#essentialFor">
      <rdfs:isDefinedBy rdf:resource="http://index.dev/ontology/rmo#tech"/>
   </rdf:Description>
   <owl:DatatypeProperty rdf:about="http://www.w3.org/ns/locn#geographicName"/>
   <rdf:Description rdf:about="http://www.w3.org/ns/locn#geographicName">
      <skos:prefLabel xml:lang="en">Geographic name</skos:prefLabel>
   </rdf:Description>
   <rdf:Description rdf:about="http://www.w3.org/ns/locn#geographicName">
      <skos:definition xml:lang="en">A textual description for a Location. (dct:Location)</skos:definition>
   </rdf:Description>
   <owl:DatatypeProperty rdf:about="http://index.dev/ontology/rmo#timeZone"/>
   <rdf:Description rdf:about="http://index.dev/ontology/rmo#timeZone">
      <skos:prefLabel xml:lang="en">Time zone</skos:prefLabel>
   </rdf:Description>
   <rdf:Description rdf:about="http://index.dev/ontology/rmo#timeZone">
      <skos:definition xml:lang="en">An area which observes a uniform standard time for legal, commercial and social purposes. (dct:Location)</skos:definition>
   </rdf:Description>
   <rdf:Description rdf:about="http://index.dev/ontology/rmo#timeZone">
      <rdfs:isDefinedBy rdf:resource="http://index.dev/ontology/rmo#tech"/>
   </rdf:Description>
   <owl:DatatypeProperty rdf:about="http://purl.org/dc/terms/description"/>
   <rdf:Description rdf:about="http://purl.org/dc/terms/description">
      <skos:prefLabel xml:lang="en">Description</skos:prefLabel>
   </rdf:Description>
   <rdf:Description rdf:about="http://purl.org/dc/terms/description">
      <skos:definition xml:lang="en">An account of the resource. Additional Information: Description may include but is not limited to: an abstract, a table of contents, a graphical representation, or a free-text account of the resource. (rmo:Benefits) An account of the resource. Additional Information: Description may include but is not limited to: an abstract, a table of contents, a graphical representation, or a free-text account of the resource. (rmo:Certification) An account of the resource. Additional Information: Description may include but is not limited to: an abstract, a table of contents, a graphical representation, or a free-text account of the resource. (rmo:Company) An account of the resource. Additional Information: Description may include but is not limited to: an abstract, a table of contents, a graphical representation, or a free-text account of the resource. (rmo:Experience) An account of the resource. Additional Information: Description may include but is not limited to: an abstract, a table of contents, a graphical representation, or a free-text account of the resource. (rmo:JobDescription) An account of the resource. Additional Information: Description may include but is not limited to: an abstract, a table of contents, a graphical representation, or a free-text account of the resource. (rmo:Qualification)</skos:definition>
   </rdf:Description>
   <owl:DatatypeProperty rdf:about="http://index.dev/ontology/rmo#BenefitName"/>
   <rdf:Description rdf:about="http://index.dev/ontology/rmo#BenefitName">
      <skos:prefLabel xml:lang="en">Benefit name</skos:prefLabel>
   </rdf:Description>
   <rdf:Description rdf:about="http://index.dev/ontology/rmo#BenefitName">
      <rdfs:isDefinedBy rdf:resource="http://index.dev/ontology/rmo#tech"/>
   </rdf:Description>
   <owl:DatatypeProperty rdf:about="http://purl.org/dc/terms/title"/>
   <rdf:Description rdf:about="http://purl.org/dc/terms/title">
      <skos:prefLabel xml:lang="en">Title</skos:prefLabel>
   </rdf:Description>
   <rdf:Description rdf:about="http://purl.org/dc/terms/title">
      <skos:definition xml:lang="en">Represents the title or the name of a resource. (rmo:Candidate) Represents the title or the name of a resource. (rmo:Credential) Represents the title or the name of a resource. (rmo:Experience) Represents the title or the name of a resource. (rmo:JobDescription) Represents the title or the name of a resource. (rmo:Qualification) Represents the title or the name of a resource. (rmo:Role) Represents the title or the name of a resource. (rmo:Skill)</skos:definition>
   </rdf:Description>
   <owl:DatatypeProperty rdf:about="http://xmlns.com/foaf/0.1/homepage"/>
   <rdf:Description rdf:about="http://xmlns.com/foaf/0.1/homepage">
      <skos:prefLabel xml:lang="en">Homepage</skos:prefLabel>
   </rdf:Description>
   <owl:DatatypeProperty rdf:about="http://xmlns.com/foaf/0.1/mbox"/>
   <rdf:Description rdf:about="http://xmlns.com/foaf/0.1/mbox">
      <skos:prefLabel xml:lang="en">Mbox</skos:prefLabel>
   </rdf:Description>
   <owl:DatatypeProperty rdf:about="http://xmlns.com/foaf/0.1/name"/>
   <rdf:Description rdf:about="http://xmlns.com/foaf/0.1/name">
      <skos:prefLabel xml:lang="en">Name</skos:prefLabel>
   </rdf:Description>
   <rdf:Description rdf:about="http://xmlns.com/foaf/0.1/name">
      <skos:definition xml:lang="en">The complete name of the Candidate as one string. (rmo:Candidate)</skos:definition>
   </rdf:Description>
   <owl:DatatypeProperty rdf:about="http://index.dev/ontology/rmo#phoneNumber"/>
   <rdf:Description rdf:about="http://index.dev/ontology/rmo#phoneNumber">
      <skos:prefLabel xml:lang="en">Phone number</skos:prefLabel>
   </rdf:Description>
   <rdf:Description rdf:about="http://index.dev/ontology/rmo#phoneNumber">
      <skos:definition xml:lang="en">A telephone number through which the Candidate can be contacted. (rmo:Candidate)</skos:definition>
   </rdf:Description>
   <rdf:Description rdf:about="http://index.dev/ontology/rmo#phoneNumber">
      <rdfs:isDefinedBy rdf:resource="http://index.dev/ontology/rmo#tech"/>
   </rdf:Description>
   <owl:DatatypeProperty rdf:about="http://index.dev/ontology/rmo#profileId"/>
   <rdf:Description rdf:about="http://index.dev/ontology/rmo#profileId">
      <skos:prefLabel xml:lang="en">Profile id</skos:prefLabel>
   </rdf:Description>
   <rdf:Description rdf:about="http://index.dev/ontology/rmo#profileId">
      <skos:definition xml:lang="en">A unique identifier for the candidate profile. (rmo:CandidateProfile)</skos:definition>
   </rdf:Description>
   <rdf:Description rdf:about="http://index.dev/ontology/rmo#profileId">
      <rdfs:isDefinedBy rdf:resource="http://index.dev/ontology/rmo#tech"/>
   </rdf:Description>
   <owl:DatatypeProperty rdf:about="http://index.dev/ontology/rmo#targetRate"/>
   <rdf:Description rdf:about="http://index.dev/ontology/rmo#targetRate">
      <skos:prefLabel xml:lang="en">Target rate</skos:prefLabel>
   </rdf:Description>
   <rdf:Description rdf:about="http://index.dev/ontology/rmo#targetRate">
      <skos:definition xml:lang="en">Specifies the desired hourly or annual rate of pay for the candidate, indicating their expected compensation for a job. (rmo:CandidateProfile)</skos:definition>
   </rdf:Description>
   <rdf:Description rdf:about="http://index.dev/ontology/rmo#targetRate">
      <rdfs:isDefinedBy rdf:resource="http://index.dev/ontology/rmo#tech"/>
   </rdf:Description>
   <owl:DatatypeProperty rdf:about="http://index.dev/ontology/rmo#companyName"/>
   <rdf:Description rdf:about="http://index.dev/ontology/rmo#companyName">
      <skos:prefLabel xml:lang="en">Company name</skos:prefLabel>
   </rdf:Description>
   <rdf:Description rdf:about="http://index.dev/ontology/rmo#companyName">
      <skos:definition xml:lang="en">The name of the organization or business entity that has posted a job description. (rmo:Company)</skos:definition>
   </rdf:Description>
   <rdf:Description rdf:about="http://index.dev/ontology/rmo#companyName">
      <rdfs:isDefinedBy rdf:resource="http://index.dev/ontology/rmo#tech"/>
   </rdf:Description>
   <owl:DatatypeProperty rdf:about="http://index.dev/ontology/rmo#industry"/>
   <rdf:Description rdf:about="http://index.dev/ontology/rmo#industry">
      <skos:prefLabel xml:lang="en">Industry</skos:prefLabel>
   </rdf:Description>
   <rdf:Description rdf:about="http://index.dev/ontology/rmo#industry">
      <rdfs:isDefinedBy rdf:resource="http://index.dev/ontology/rmo#tech"/>
   </rdf:Description>
   <owl:DatatypeProperty rdf:about="http://index.dev/ontology/rmo#dateAwarded"/>
   <rdf:Description rdf:about="http://index.dev/ontology/rmo#dateAwarded">
      <skos:prefLabel xml:lang="en">Date awarded</skos:prefLabel>
   </rdf:Description>
   <rdf:Description rdf:about="http://index.dev/ontology/rmo#dateAwarded">
      <skos:definition xml:lang="en">The date when a candidate was granted a particular credential, such as a degree or certification. (rmo:Credential)</skos:definition>
   </rdf:Description>
   <rdf:Description rdf:about="http://index.dev/ontology/rmo#dateAwarded">
      <rdfs:isDefinedBy rdf:resource="http://index.dev/ontology/rmo#tech"/>
   </rdf:Description>
   <owl:DatatypeProperty rdf:about="http://index.dev/ontology/rmo#educationDegree"/>
   <rdf:Description rdf:about="http://index.dev/ontology/rmo#educationDegree">
      <skos:prefLabel xml:lang="en">Education degree</skos:prefLabel>
   </rdf:Description>
   <rdf:Description rdf:about="http://index.dev/ontology/rmo#educationDegree">
      <rdfs:isDefinedBy rdf:resource="http://index.dev/ontology/rmo#tech"/>
   </rdf:Description>
   <rdf:Property rdf:about="http://index.dev/ontology/rmo#yearsOfExperience"/>
   <rdf:Description rdf:about="http://index.dev/ontology/rmo#yearsOfExperience">
      <skos:prefLabel xml:lang="en">Years of experience</skos:prefLabel>
   </rdf:Description>
   <rdf:Description rdf:about="http://index.dev/ontology/rmo#yearsOfExperience">
      <skos:definition xml:lang="en">Indicates the total number of years a candidate has worked in their field or occupation. (rmo:Experience)</skos:definition>
   </rdf:Description>
   <rdf:Description rdf:about="http://index.dev/ontology/rmo#yearsOfExperience">
      <rdfs:isDefinedBy rdf:resource="http://index.dev/ontology/rmo#tech"/>
   </rdf:Description>
   <owl:DatatypeProperty rdf:about="http://index.dev/ontology/rmo#availability"/>
   <rdf:Description rdf:about="http://index.dev/ontology/rmo#availability">
      <skos:prefLabel xml:lang="en">Availability</skos:prefLabel>
   </rdf:Description>
   <rdf:Description rdf:about="http://index.dev/ontology/rmo#availability">
      <skos:definition xml:lang="en">Indicates when the job position is open for applications, including specific dates or time frames such as "immediate" or "within three months." (rmo:JobDescription)</skos:definition>
   </rdf:Description>
   <rdf:Description rdf:about="http://index.dev/ontology/rmo#availability">
      <rdfs:isDefinedBy rdf:resource="http://index.dev/ontology/rmo#tech"/>
   </rdf:Description>
   <owl:DatatypeProperty rdf:about="http://index.dev/ontology/rmo#jobId"/>
   <rdf:Description rdf:about="http://index.dev/ontology/rmo#jobId">
      <skos:prefLabel xml:lang="en">Job id</skos:prefLabel>
   </rdf:Description>
   <rdf:Description rdf:about="http://index.dev/ontology/rmo#jobId">
      <skos:definition xml:lang="en">A unique identifier for a job description, used to distinguish it from other job description. (rmo:JobDescription)</skos:definition>
   </rdf:Description>
   <rdf:Description rdf:about="http://index.dev/ontology/rmo#jobId">
      <rdfs:isDefinedBy rdf:resource="http://index.dev/ontology/rmo#tech"/>
   </rdf:Description>
   <owl:DatatypeProperty rdf:about="http://index.dev/ontology/rmo#projectType"/>
   <rdf:Description rdf:about="http://index.dev/ontology/rmo#projectType">
      <skos:prefLabel xml:lang="en">Project type</skos:prefLabel>
   </rdf:Description>
   <rdf:Description rdf:about="http://index.dev/ontology/rmo#projectType">
      <skos:definition xml:lang="en">Represents the nature or category of a project, such as software development, research, or marketing. (rmo:JobDescription)</skos:definition>
   </rdf:Description>
   <rdf:Description rdf:about="http://index.dev/ontology/rmo#projectType">
      <rdfs:isDefinedBy rdf:resource="http://index.dev/ontology/rmo#tech"/>
   </rdf:Description>
   <owl:DatatypeProperty rdf:about="http://index.dev/ontology/rmo#rate"/>
   <rdf:Description rdf:about="http://index.dev/ontology/rmo#rate">
      <skos:prefLabel xml:lang="en">Rate</skos:prefLabel>
   </rdf:Description>
   <rdf:Description rdf:about="http://index.dev/ontology/rmo#rate">
      <skos:definition xml:lang="en">Specifies the compensation for the job, typically expressed as an hourly rate, salary, or contract amount. (rmo:JobDescription)</skos:definition>
   </rdf:Description>
   <rdf:Description rdf:about="http://index.dev/ontology/rmo#rate">
      <rdfs:isDefinedBy rdf:resource="http://index.dev/ontology/rmo#tech"/>
   </rdf:Description>
   <rdf:Property rdf:about="http://index.dev/ontology/rmo#startDate"/>
   <rdf:Description rdf:about="http://index.dev/ontology/rmo#startDate">
      <skos:prefLabel xml:lang="en">Start date</skos:prefLabel>
   </rdf:Description>
   <rdf:Description rdf:about="http://index.dev/ontology/rmo#startDate">
      <skos:definition xml:lang="en">Represents the date when a job description, project, or engagement is scheduled to begin. (rmo:JobDescription)</skos:definition>
   </rdf:Description>
   <rdf:Description rdf:about="http://index.dev/ontology/rmo#startDate">
      <rdfs:isDefinedBy rdf:resource="http://index.dev/ontology/rmo#tech"/>
   </rdf:Description>
   <owl:DatatypeProperty rdf:about="http://www.w3.org/2004/02/skos/core#altLabel"/>
   <rdf:Description rdf:about="http://www.w3.org/2004/02/skos/core#altLabel">
      <skos:prefLabel xml:lang="en">Alt label</skos:prefLabel>
   </rdf:Description>
   <rdf:Description rdf:about="http://www.w3.org/2004/02/skos/core#altLabel">
      <skos:definition xml:lang="en">An alternative lexical label for a resource. Acronyms, abbreviations, spelling variants, and irregular plural/singular forms may be included among the alternative labels for a concept. (rmo:Qualification) An alternative lexical label for a resource. Acronyms, abbreviations, spelling variants, and irregular plural/singular forms may be included among the alternative labels for a concept. (rmo:Skill) An alternative lexical label for a resource. Acronyms, abbreviations, spelling variants, and irregular plural/singular forms may be included among the alternative labels for a concept. (rmo:TypeOfEngagement)</skos:definition>
   </rdf:Description>
   <rdf:Property rdf:about="http://www.w3.org/2004/02/skos/core#prefLabel"/>
   <rdf:Description rdf:about="http://www.w3.org/2004/02/skos/core#prefLabel">
      <skos:prefLabel xml:lang="en">Pref label</skos:prefLabel>
   </rdf:Description>
   <rdf:Description rdf:about="http://www.w3.org/2004/02/skos/core#prefLabel">
      <skos:definition xml:lang="en">The preferred lexical label for a resource, in a given language. (rmo:Qualification) The preferred lexical label for a resource, in a given language. (rmo:Skill)</skos:definition>
   </rdf:Description>
   <owl:DatatypeProperty rdf:about="http://index.dev/ontology/rmo#yearsOfSkill"/>
   <rdf:Description rdf:about="http://index.dev/ontology/rmo#yearsOfSkill">
      <skos:prefLabel xml:lang="en">Years of skill</skos:prefLabel>
   </rdf:Description>
   <rdf:Description rdf:about="http://index.dev/ontology/rmo#yearsOfSkill">
      <skos:definition xml:lang="en">Indicates the number of years a candidate has utilized a specific skill. (rmo:Skill)</skos:definition>
   </rdf:Description>
   <rdf:Description rdf:about="http://index.dev/ontology/rmo#yearsOfSkill">
      <rdfs:isDefinedBy rdf:resource="http://index.dev/ontology/rmo#tech"/>
   </rdf:Description>
   <owl:DatatypeProperty rdf:about="http://index.dev/ontology/rmo#engagementType"/>
   <rdf:Description rdf:about="http://index.dev/ontology/rmo#engagementType">
      <skos:prefLabel xml:lang="en">Engagement type</skos:prefLabel>
   </rdf:Description>
   <rdf:Description rdf:about="http://index.dev/ontology/rmo#engagementType">
      <skos:definition xml:lang="en">It includes part-time, full-time, or contractual roles. (rmo:TypeOfEngagement)</skos:definition>
   </rdf:Description>
   <rdf:Description rdf:about="http://index.dev/ontology/rmo#engagementType">
      <rdfs:isDefinedBy rdf:resource="http://index.dev/ontology/rmo#tech"/>
   </rdf:Description>
</rdf:RDF>
